theories/Dot/typing/typingStamping.v
@@ -1,4 +1,5 @@
-From D.Dot Require Import typing_stamped stampingDefsCore astStamping skeleton syn.path_repl.
+From D.Dot Require Import typing_stamped stampingDefsCore astStamping skeleton
+  path_repl_lemmas.
 From D.Dot Require typing_unstamped.
 
 Set Implicit Arguments.
@@ -70,6 +71,14 @@ Section syntyping_stamping_lemmas.
   Hint Resolve is_stamped_path2tm is_unstamped_path2tm unstamp_path2tm : core.
   Hint Resolve unstamped_stamped_path unstamped_stamps_self_path : core.
 
+  Hint Resolve psubst_one_implies is_unstamped_ty_subst : core.
+  (** These hints slow down proof search. *)
+  (** Not directed. *)
+  Remove Hints typing_stamped.psingleton_trans : core.
+  (** These cause cycles. *)
+  Remove Hints typing_stamped.p_mu_e_typed : core.
+  Remove Hints typing_stamped.p_mu_i_typed : core.
+
   Lemma stamp_objIdent_typing_mut Γ :
     (∀ e T, Γ u⊢ₜ e : T →
       ∀ (g : stys), ∃ e' (g' : stys),
@@ -114,20 +123,23 @@ Section syntyping_stamping_lemmas.
     all: try solve [intros * Hu1 IHs1 **; move: IHs1 => /(.$ g) [g1 [Hts1 Hle1]]; exists g1; split_and!; eauto 3].
     all: try solve [intros; exists g; split_and!; auto 3].
 
-  - intros * Hu1 IHs1 Hu2 IHs2 g.
+  (* - intros * Hu1 IHs1 Hu2 IHs2 g.
     move: IHs1 => /(.$ g) [e1' [g1 ?]];
     move: IHs2 => /(.$ g1) [e2' [g2 ?]]; ev; lte g g1 g2.
     exists (tapp e1' (tv (var_vl x2))), g2.
     (* Expressions that appear in types must stamp to themselves! *)
     suff ?: e2' = tv (var_vl x2) by naive_solver.
-    destruct e2'; naive_solver.
-  - intros * Hps Hus1 Hu1 IHs1 Hu2 IHs2 g.
+    destruct e2'; naive_solver. *)
+  - intros * Hus1 Husp Hu1 IHs1 Hu2 IHs2 g.
     move: IHs1 => /(.$ g) [e1' [g1 [IHs1 [Hle1 Hse1]]]];
     move: IHs2 => /(.$ g1) [p2' [g2 [IHs2 [Hle2 ?]]]]; lte g g1 g2.
     have Hse1': unstamp_tm g2 e1' = e1. by eapply stamps_unstamp_mono_tm, Hse1.
     have ?: p2' = p2. move: (unstamped_path_root_is_var Hu2). naive_solver.
     subst p2'.
     exists (tapp e1' (path2tm p2)), g2.
+    (* have ?: T2 .Tp[ p2 /]~ psubst_one_ty T2 p2 by exact: psubst_one_implies.
+    have ?: is_unstamped_ty (length Γ) (psubst_one_ty T2 p2)
+      by eapply is_unstamped_ty_subst. *)
     split_and!; first eapply typing_stamped.App_path_typed; naive_solver eauto 4.
   - intros * Hu1 IHs1 Hu2 IHs2 g.
     move: IHs1 => /(.$ g) [e1' [g1 ?]];
@@ -136,22 +148,22 @@ Section syntyping_stamping_lemmas.
   - intros * Hu1 IHs1 g.
     move: IHs1 => /(.$ g) [e1' [g1 ?]].
     exists (tproj e1' l), g1; naive_solver.
-  - intros * Hu1 IHs1 g.
+  (* - intros * Hu1 IHs1 g.
     move: IHs1 => /(.$ g) [e1' [g1 ?]].
     exists (tv (var_vl x)), g1.
     suff ?: e1' = tv (var_vl x) by naive_solver.
-    destruct e1'; naive_solver.
+    destruct e1'; naive_solver. *)
   - intros * Hus1 Hu1 IHs1 g.
     move: IHs1 => /(.$ g) [e' [g1 ?]].
     exists (tv (vabs e')), g1. naive_solver.
   - intros * Huds1 IHs1 Hus1 g.
     move: IHs1 => /(.$ g) [ds' [g1 ?]].
     exists (tv (vobj ds')), g1; naive_solver.
-  - intros * Hu1 IHs1 g.
+  (* - intros * Hu1 IHs1 g.
     move: IHs1 => /(.$ g) [e1' [g1 ?]].
     exists (tv (var_vl x)), g1.
     suff ?: e1' = tv (var_vl x) by naive_solver.
-    destruct e1'; naive_solver.
+    destruct e1'; naive_solver. *)
   - intros. exists (tv (vnat n)), g; naive_solver.
   - intros.
     have ? : x < length Γ by exact: lookup_lt_Some.
@@ -225,13 +237,15 @@ Section syntyping_stamping_lemmas.
     exists p1', g2.
     split_and! => //. eapply typing_stamped.p_subs_typed, IHs2.
     by eapply stamped_objIdent_subtype_mono, Hs1.
-  - intros * Hps Hus Hu1 IHs1 g.
+  - intros * Hus Hu1 IHs1 g.
     move: IHs1 => /(.$ g) /= [p1' [g1 ?]]; ev.
-    exists p1', g1. suff ?: p1' = p by naive_solver.
+    exists p1', g1.
+    suff ?: p1' = p by split_and! => //; econstructor; naive_solver.
     move: (unstamped_path_root_is_var Hu1). naive_solver.
-  - intros * Hps Hus1 Hu1 IHs1 g.
+  - intros * Hus1 Hu1 IHs1 g.
     move: IHs1 => /(.$ g) /= [p1' [g1 [IHs1 ?]]]; ev.
-    exists p1', g1. suff ?: p1' = p by naive_solver.
+    exists p1', g1.
+    suff ?: p1' = p by split_and! => //; econstructor; naive_solver.
     move: (unstamped_path_root_is_var Hu1). naive_solver.
   - intros * Hu1 IHs1 g.
     move: IHs1 => /(.$ g) /= [p1' [g1 [IHs1 ?]]]; ev.
